Show that only one value will be chosen in a full execution.
This change introduces the concept of a state being "reachable from"
another state. The relevance is that for two states to be "in the same
execution", one must be reachable (from an initial state) and the
other must be reachable from the first.

Under the assumption that `voted` is a stable predicate, we show that
if a state `dst` is reachable from a reachable state `src`, and values
are chosen at `src` and `dst`, then both chosen values must be the
same. The argument is that the stability of `voted` implies the
stability of `chosen`, so if a value is chosen at `src`, it is also
chosen at `dst`. The first safety theorem shows that both values
are the same.

src/guidelines/multipaxos.lean
@@ -88,6 +88,9 @@ structure proto_constraints
         proto.next state s' →
           defs.voted s' process slot ballot →
             defs.voted state process slot ballot ∨ defs.curr state process ≤ ballot))
+  (voted_stable :
+    ∀ process slot ballot,
+      proto.stable (λ state, defs.voted state process slot ballot))
   (voted_imp_proposed :
     ∀ process slot ballot,
       proto.invariant (λ state,
@@ -118,27 +121,30 @@ def safety (proto : protocol sys_state_t)
   (defs : state_defs sys_state_t pid_t slot_t ballot_t value_t)
   := proto.invariant (λ state, (∀ slot v v', defs.chosen state slot v → defs.chosen state slot v' → v = v'))
 
+def safety_v2 (proto : protocol sys_state_t)
+  (defs : state_defs sys_state_t pid_t slot_t ballot_t value_t)
+  := proto.invariant (λ state, (∀ later_state slot v v', proto.reachable_from state later_state →
+                                  defs.chosen state slot v → defs.chosen later_state slot v' → v = v'))
+
 end multipaxos
 
+variables (sys_state_t pid_t slot_t ballot_t value_t : Type)
+          [linear_order ballot_t] [decidable_eq pid_t] (proto : protocol sys_state_t)
+          (defs : multipaxos.state_defs sys_state_t pid_t slot_t ballot_t value_t)
 
-variables {sys_state_t pid_t slot_t ballot_t value_t : Type}
-          [linear_order ballot_t] [decidable_eq pid_t]
-          {proto : protocol sys_state_t}
-          {defs : multipaxos.state_defs sys_state_t pid_t slot_t ballot_t value_t}
-
-theorem constraints_give_safety : multipaxos.proto_constraints proto defs → multipaxos.safety proto defs :=
-begin
-intro multipaxos_constraints_met,
-suffices key : ∀ slot, proto.invariant (λ state, (∀ v v', defs.chosen state slot v → defs.chosen state slot v' → v = v')),
-by { intros state reachable slot, exact key slot state reachable },
-intro slot,
-let slot_instance_defs : paxos_defs sys_state_t pid_t ballot_t value_t :=
+-- Given a multipaxos algorithm, we can restrict to a single slot to get a
+-- single-instance paxos algorithm.
+def slot_instance_defs (slot : slot_t): paxos_defs sys_state_t pid_t ballot_t value_t :=
 { curr := λ state p, defs.curr state p,
   stored := λ state p, defs.stored state p slot,
   proposed := λ state ballot value, defs.proposed state slot ballot value,
   voted := λ state p ballot, defs.voted state p slot ballot,
-  quorum := defs.quorum },
-let slot_instance_reqs_sat : requirements proto slot_instance_defs :=
+  quorum := defs.quorum }
+
+-- The single-instance paxos algorithm obtained in this way meets the safety
+-- constraints.
+def slot_instance_reqs_sat (multipaxos_constraints_met : multipaxos.proto_constraints proto defs) (slot : slot_t)
+  : requirements proto (slot_instance_defs sys_state_t pid_t slot_t ballot_t value_t defs slot) :=
 { quorums_intersect := multipaxos_constraints_met.quorums_intersect,
   none_proposed_at_init := λ state ballot value is_init,
     multipaxos_constraints_met.none_proposed_at_init state slot ballot value is_init,
@@ -155,12 +161,14 @@ let slot_instance_reqs_sat : requirements proto slot_instance_defs :=
     multipaxos_constraints_met.stored_is_proposed process slot prop,
   new_votes_ge_curr_ballot := λ process ballot s',
     multipaxos_constraints_met.new_votes_ge_curr_ballot process slot ballot s',
+  voted_stable := λ process ballot,
+    multipaxos_constraints_met.voted_stable process slot ballot,
   voted_imp_proposed := λ process ballot,
     multipaxos_constraints_met.voted_imp_proposed process slot ballot,
   voted_le_stored := λ process ballot,
     multipaxos_constraints_met.voted_le_stored process slot ballot,
   majority_have_upper_interval_if_proposed := by {
-    suffices key : (proto_with_intervals_recorded slot_instance_defs proto).invariant
+    suffices key : (proto_with_intervals_recorded (slot_instance_defs sys_state_t pid_t slot_t ballot_t value_t defs slot) proto).invariant
       (λ restricted_state,
         ∃ full_state, (multipaxos.state_with_past_intervals defs proto).reachable full_state ∧
                       full_state.fst = restricted_state.fst ∧
@@ -194,7 +202,25 @@ let slot_instance_reqs_sat : requirements proto slot_instance_defs :=
     { refl },
     rw function.funext_iff, intro p,
     rw next_reachable.right p, unfold prod.snd,
-    rw lift_snd_restriction_gives_snd
-  } },
-exact requirements_give_safety slot_instance_reqs_sat
+    rw lift_snd_restriction_gives_snd,
+    unfold slot_instance_defs
+  } }
+
+theorem constraints_give_safety : multipaxos.proto_constraints proto defs → multipaxos.safety proto defs :=
+begin
+intro multipaxos_constraints_met,
+suffices key : ∀ slot, proto.invariant (λ state, (∀ v v', defs.chosen state slot v → defs.chosen state slot v' → v = v')),
+by { intros state reachable slot, exact key slot state reachable },
+intro slot,
+exact requirements_give_safety (slot_instance_reqs_sat sys_state_t pid_t slot_t ballot_t value_t proto defs multipaxos_constraints_met slot)
+end
+
+theorem constraints_give_safety_v2 : multipaxos.proto_constraints proto defs → multipaxos.safety_v2 proto defs :=
+begin
+intro multipaxos_constraints_met,
+suffices key : ∀ slot, proto.invariant (λ state, (∀ later_state v v', proto.reachable_from state later_state →
+                                                    defs.chosen state slot v → defs.chosen later_state slot v' → v = v')),
+by { intros state reachable later_state slot, exact key slot state reachable later_state },
+intro slot,
+exact requirements_give_safety_v2 (slot_instance_reqs_sat sys_state_t pid_t slot_t ballot_t value_t proto defs multipaxos_constraints_met slot)
 end
