src/guidelines/protocol.lean
@@ -15,6 +15,14 @@ def reachable_in (proto : protocol sys_state_t) : ℕ → sys_state_t → Prop
 def reachable (proto : protocol sys_state_t) (s : sys_state_t) :=
   ∃ n, reachable_in proto n s
 
+def reachable_in_from (proto : protocol sys_state_t) (src : sys_state_t) : ℕ → sys_state_t → Prop
+| 0       := (λ dst, dst = src)
+| (n + 1) := (λ dst, (∃ intermediate, reachable_in_from n intermediate ∧
+                                      proto.next intermediate dst))
+
+def reachable_from (proto : protocol sys_state_t) (src dst : sys_state_t) :=
+  ∃ n, reachable_in_from proto src n dst
+
 def invariant (proto : protocol sys_state_t) (predicate : sys_state_t → Prop) :=
   ∀ s, reachable proto s → predicate s
 
@@ -41,6 +49,35 @@ induction n with k hk,
 { intros s s_r_zero, exact holds_at_init s s_r_zero },
 rintros s ⟨u, u_r_k, u_next_s⟩,
 exact inductive_step u ⟨k, u_r_k⟩ s (hk u u_r_k) u_next_s
+end
+
+lemma reachable_from_reachable_is_reachable (proto : protocol sys_state_t) :
+  ∀ s s', proto.reachable s → proto.reachable_from s s' → proto.reachable s' :=
+begin
+suffices : ∀ s, proto.reachable s → ∀ n s', proto.reachable_in_from s n s' → proto.reachable s',
+by { rintros s s' reachable_s ⟨n, s'_reachable_from_s_in_n⟩, exact this s reachable_s n s' s'_reachable_from_s_in_n },
+intros s reachable_s n,
+induction n with k hk,
+{ intros s' hs',
+  have : s' = s := hs', rw this, exact reachable_s },
+rintros s'' ⟨s', s'_reachable_from_s_in_k, s''_follows_s'⟩,
+rcases (hk s' s'_reachable_from_s_in_k) with ⟨j, hj⟩,
+exact ⟨j.succ, s', hj, s''_follows_s'⟩
+end
+
+lemma stability_applies_to_reachable_from (predicate : sys_state_t → Prop)
+  (proto : protocol sys_state_t) :
+  proto.stable predicate → ∀ s s', proto.reachable_from s s' → predicate s → predicate s' :=
+begin
+intro stability,
+suffices : ∀ n s, predicate s → ∀ s', proto.reachable_in_from s n s' → predicate s',
+by {
+  rintros s s' ⟨n, hn⟩ predicate_at_s,
+  exact this n s predicate_at_s s' hn },
+intros n s predicate_at_s, induction n with k hk,
+{ intros s' h, have : s' = s := h, rw this, exact predicate_at_s },
+rintros s'' ⟨s', s'_reachable_in_k, s''_follows_s'⟩,
+exact stability s' s'' (hk s' s'_reachable_in_k) s''_follows_s',
 end
 
 end protocol
